theories/c_toy_mlang/adequacy.v
@@ -1,0 +1,159 @@
+From iris.algebra Require Import gmap auth agree gset coPset.
+From iris.proofmode Require Import proofmode.
+From iris.base_logic.lib Require Import wsat.
+From melocoton.language Require Import mlanguage.
+From melocoton.c_toy_mlang Require Import weakestpre.
+From melocoton Require Import multirelations.
+
+Section adequacy.
+Context `{!irisGS_gen hlc Λ Σ}.
+Implicit Types e : expr Λ.
+Implicit Types P Q : iProp Σ.
+Implicit Types Φ : val Λ → iProp Σ.
+Implicit Types φ : expr Λ * state Λ → Prop.
+
+Lemma wp_step p e1 σ1 ns φ Φ :
+  rel (prim_step p) (e1, σ1) φ →
+  state_interp σ1 ns -∗
+  £ (S (num_laters_per_step ns)) -∗
+  WP e1 @ p; ⊤ {{ Φ }}
+    ={⊤,∅}=∗ |={∅}▷=>^(S $ num_laters_per_step ns) |={∅,⊤}=>
+    ∃ e2 σ2,
+      ⌜φ (e2, σ2)⌝ ∗ state_interp σ2 (S ns) ∗ WP e2 @ p; ⊤ {{ Φ }}.
+Proof using.
+  rewrite {1}wp_unfold /wp_pre. iIntros (?) "Hσ Hcred H".
+  rewrite (val_stuck p e1 σ1 φ) //.
+  iMod ("H" $! σ1 ns with "Hσ") as "(_ & H)". iModIntro.
+  iApply (step_fupdN_wand with "(H [//] Hcred)"). iIntros ">H".
+  iDestruct "H" as (e2 σ2 Hφ) "(? & ?)". by eauto with iFrame.
+Qed.
+
+Local Fixpoint steps_sum (num_laters_per_step : nat → nat) (start ns : nat) : nat :=
+  match ns with
+  | O => 0
+  | S ns =>
+    S $ num_laters_per_step start + steps_sum num_laters_per_step (S start) ns
+  end.
+
+Lemma wp_steps p n e1 σ1 ns φ Φ :
+  rel (repeat (prim_step p) n) (e1, σ1) φ →
+  state_interp σ1 ns -∗
+  £ (steps_sum num_laters_per_step ns n) -∗
+  WP e1 @ p; ⊤ {{ Φ }}
+    ={⊤,∅}=∗ |={∅}▷=>^(steps_sum num_laters_per_step ns n) |={∅,⊤}=>
+    ∃ e2 σ2,
+      ⌜φ (e2, σ2)⌝ ∗
+      state_interp σ2 (n + ns) ∗
+      WP e2 @ p; ⊤ {{ Φ }}.
+Proof using.
+  revert e1 σ1 ns φ Φ.
+  induction n as [|n IH]=> e1 σ1 ns φ Φ /=.
+  { unfold id, rel; cbn. iIntros (Hφ) "Hσ ? Hwp".
+    iApply fupd_mask_intro. done. iIntros "H"; iMod "H".
+    iModIntro. iExists e1, σ1. eauto with iFrame. }
+  iIntros (Hsteps) "Hσ Hcred He".
+  rewrite unfold_seq in Hsteps.
+  destruct Hsteps as (φ' & Hstep1 & Hstep2).
+  rewrite Nat.iter_add -{1}plus_Sn_m plus_n_Sm.
+  rewrite lc_split. iDestruct "Hcred" as "[Hc1 Hc2]".
+  iDestruct (wp_step with "Hσ Hc1 He") as ">H"; first eauto.
+  iModIntro. iApply step_fupdN_S_fupd. iApply (step_fupdN_wand with "H").
+  iIntros ">H". iDestruct "H" as (e2 σ2 Hφ) "(Hσ & He)".
+  iMod (IH with "Hσ Hc2 He") as "IH"; first eauto. iModIntro.
+  iApply (step_fupdN_wand with "IH"). iIntros ">IH".
+  iDestruct "IH" as (e3 σ3 Hφ') "[??]".
+  by eauto with iFrame.
+Qed.
+
+Local Lemma wp_strong_adequacy_internal p n e1 σ1 ns φ Φ :
+  rel (repeat (prim_step p) n) (e1, σ1) φ →
+  state_interp σ1 ns -∗
+  £ (steps_sum num_laters_per_step ns n) -∗
+  WP e1 @ p; ⊤ {{ Φ }}
+    ={⊤,∅}=∗ |={∅}▷=>^(steps_sum num_laters_per_step ns n) |={∅,⊤}=>
+    ∃ e2 σ2,
+      ⌜φ (e2, σ2)⌝ ∗
+      state_interp σ2 (n + ns) ∗
+      from_option Φ True (to_val e2).
+Proof using.
+  iIntros (Hstep) "Hσ Hcred He". iMod (wp_steps with "Hσ Hcred He") as "Hwp"; first done.
+  iModIntro. iApply (step_fupdN_wand with "Hwp").
+  iMod 1 as (? ? ?) "(Hσ & He)".
+  destruct (to_val e2) as [v2|] eqn:He2.
+  { apply of_to_val in He2 as <-. simpl. rewrite wp_value_fupd'.
+    iMod "He". iModIntro. iExists _, _. iFrame. iSplit; eauto.
+    rewrite to_of_val //. }
+  { iModIntro. iExists _, _. iFrame. iSplit; eauto. rewrite He2//. }
+Qed.
+End adequacy.
+
+Lemma wp_strong_adequacy_gen (hlc : has_lc) Σ Λ `{!invGpreS Σ} p e1 σ1 n φ P
+        (num_laters_per_step : nat → nat) :
+  (∀ `{Hinv : !invGS_gen hlc Σ},
+     ⊢ |={⊤}=> ∃
+        (stateI : state Λ → nat → iProp Σ)
+        (Φ : val Λ → iProp Σ)
+        state_interp_mono,
+     let _ : irisGS_gen hlc Λ Σ := IrisG Hinv stateI num_laters_per_step state_interp_mono in
+     stateI σ1 0 ∗
+     WP e1 @ p; ⊤ {{ Φ }} ∗
+     (∀ e2 σ2,
+        ⌜φ (e2, σ2)⌝ -∗
+        stateI σ2 n -∗
+        from_option Φ True (to_val e2) -∗
+        |={⊤,∅}=> ⌜ P ⌝)) →
+  rel (repeat (prim_step p) n) (e1, σ1) φ →
+  P.
+Proof.
+  iIntros (Hwp ?).
+  eapply (step_fupdN_soundness_gen _ hlc (steps_sum num_laters_per_step 0 n)
+    (steps_sum num_laters_per_step 0 n)).
+  iIntros (Hinv) "Hcred".
+  iMod Hwp as (stateI Φ state_interp_mono) "(Hσ & Hwp & HP)".
+  iMod (@wp_strong_adequacy_internal _ _ _
+        (IrisG Hinv stateI num_laters_per_step state_interp_mono)
+    with "[Hσ] Hcred Hwp") as "H"; [done|done|].
+  iAssert (|={∅}▷=>^(steps_sum num_laters_per_step 0 n) |={∅}=> ⌜P⌝)%I
+    with "[-]" as "H"; last first.
+  { destruct steps_sum; [done|]. by iApply step_fupdN_S_fupd. }
+  iApply (step_fupdN_wand with "H").
+  iMod 1 as (e2 σ2 Hφ) "(Hσ & Hval) /=".
+  rewrite -plus_n_O.
+  by iApply ("HP" with "[//] Hσ").
+Qed.
+
+(** Adequacy when using later credits (the default) *)
+Definition wp_strong_adequacy := wp_strong_adequacy_gen HasLc.
+Global Arguments wp_strong_adequacy _ _ {_}.
+
+Definition adequate {Λ} (p : program Λ) (e1 : expr Λ) (σ1 : state Λ)
+    (P : val Λ → state Λ → Prop) :=
+  ∀ φ, rel (star (prim_step p)) (e1, σ1) φ →
+       ∃ e2 σ2,
+         φ (e2, σ2) ∧
+         (∀ v2, to_val e2 = Some v2 → P v2 σ2).
+(* and recall that [∀ e2 σ2, not_stuck p e2 σ2] *)
+
+Lemma wp_adequacy_gen (hlc : has_lc) Σ Λ `{!invGpreS Σ} p e σ P :
+  (∀ `{Hinv : !invGS_gen hlc Σ},
+     ⊢ |={⊤}=> ∃ (stateI : state Λ → iProp Σ),
+       let _ : irisGS_gen hlc Λ Σ :=
+           IrisG Hinv (λ σ _, stateI σ) (λ _, 0)
+                 (λ _ _, fupd_intro _ _)
+       in
+       stateI σ ∗ WP e @ p; ⊤ {{ v, ⌜P v⌝ }}) →
+  adequate p e σ (λ v _, P v).
+Proof.
+  intros Hwp. intros φ. rewrite /rel /star /=.
+  intros [n Hsteps].
+  eapply (wp_strong_adequacy_gen hlc Σ _); [ | done]=> ?.
+  iMod Hwp as (stateI) "[Hσ Hwp]".
+  iExists (λ σ _, stateI σ), (λ v, ⌜P v⌝%I), _ => /=.
+  iIntros "{$Hσ $Hwp} !>" (e2 σ2 Hφ) "H Hv".
+  iApply fupd_mask_intro_discard; [done|].
+  iExists _, _. iSplit; eauto. iIntros (? ->). done.
+Qed.
+
+(** Instance for using credits *)
+Definition wp_adequacy := wp_adequacy_gen HasLc.
+Global Arguments wp_adequacy _ _ {_}.
