theories/c_toy_mlang/notation.v
@@ -60,8 +60,8 @@ Notation "'while:' e1 'do' e2" := (While e1%E e2%E)
 Notation "'call' ff '(' e1 , .. , en ')'" := (FunCall ff (cons e1 .. (cons en nil) ..))
   (at level 200, ff, e1, en at level 200) : expr_scope.
 
-Notation "'extern' ff '(' e1 , .. , en ')'" := (Extern ff (cons e1 .. (cons en nil) ..))
-  (at level 200, ff, e1, en at level 200) : expr_scope.
+(* Notation "'extern' ff '(' e1 , .. , en ')'" := (Extern ff (cons e1 .. (cons en nil) ..)) *)
+(*   (at level 200, ff, e1, en at level 200) : expr_scope. *)
 
 
 
